Source/PS.v
@@ -901,17 +901,15 @@ Proof.
       filterm (fun (k : nat) (_ : ComponentMemory.t) => k \notin domm (prog_buffers p1))
                     (mapm
                        (fun bufs =>
-                          let '(pub, priv):= bufs in
                           ComponentMemory.prealloc
-                            (setm (setm emptym Block.local pub) Block.private priv))
+                            (get_buffers_as_map bufs))
                        (unionm (prog_buffers p) (prog_buffers p1)))
       =
       filterm (fun (k : nat) (_ : ComponentMemory.t) => k \notin domm (prog_buffers p1))
                     (mapm
                        (fun bufs =>
-                         let '(pub, priv):= bufs in
                          ComponentMemory.prealloc
-                           (setm (setm emptym Block.local pub) Block.private priv))
+                           (get_buffers_as_map bufs))
                        (unionm (prog_buffers p) (prog_buffers p2)))
     ) as Hmem.
   {
@@ -927,9 +925,8 @@ Proof.
         rewrite fdisjointC in Hdisjoint1.
         pose proof (domm_map
                       (fun initial_buffers =>
-                           let '(pub, priv):= initial_buffers in
                            ComponentMemory.prealloc
-                             (setm (setm emptym Block.local pub) Block.private priv))
+                             (get_buffers_as_map initial_buffers))
                    (prog_buffers p))
           as Hdomm.
         rewrite <- Hdomm in Hdisjoint1.
